VProg notations

Test/VProg.v
@@ -7,234 +7,183 @@ Import SLNotations.
 Import ListNotations.
 Import DTuple.Notations.
 Import VProg._Abbrev.
+Import VProg.Notations.
 
-Definition f_0 : fid := 0.
-Definition f_1 : fid := 0.
-Definition f_2 : fid := 2.
-Definition f_3 : fid := 3.
-Definition f_4 : fid := 4.
-
-Definition sig_0 := mk_f_sig (ptr * ptr) unit.
-Definition sig_1 := mk_f_sig (ptr * ptr * ptr) unit.
-Definition sig_2 := mk_f_sig (ptr * ptr * ptr) ptr.
-Definition sig_3 := mk_f_sig ptr ptr.
-Definition sig_4 := mk_f_sig (ptr * ptr) ptr.
-
-Definition SIG : sig_context :=
-  fun f => match f with
-  | 0 => Some sig_0
-  | 1 => Some sig_1
-  | 2 => Some sig_2
-  | 3 => Some sig_3
-  | 4 => Some sig_4
-  | _ => None
-  end.
-
-Definition sigh_0 := mk_f_sigh sig_0 None None.
-Definition spec_0 : FSpec sigh_0 (fun '(p0, p1) =>
-  Spec.Expanded.mk_r0 (fun '(n0, n1) =>
-  Spec.Expanded.mk_r1 [] [CTX.mka (SLprop.cell p0, n0); CTX.mka (SLprop.cell p1, n1)] True (fun _ =>
-  Spec.Expanded.mk_r2 (fun 'tt =>
-  Spec.Expanded.mk_r3 [CTX.mka (SLprop.cell p0, n1); CTX.mka (SLprop.cell p1, n0)] True)))).
-Proof. Tac.build_FSpec. Defined.
-
-Definition sigh_1 := mk_f_sigh sig_1 None None.
-Definition spec_1 : FSpec sigh_1 (fun '(p0, p1, p2) =>
-  Spec.Expanded.mk_r0 (fun '(n0, n1, n2) =>
-  Spec.Expanded.mk_r1 [CTX.mka (SLprop.cell p2, n2)]
-    [CTX.mka (SLprop.cell p0, n0); CTX.mka (SLprop.cell p1, n1)] True (fun _ =>
-  Spec.Expanded.mk_r2 (fun 'tt =>
-  Spec.Expanded.mk_r3 [CTX.mka (SLprop.cell p0, n1); CTX.mka (SLprop.cell p1, n0)] True)))).
-Proof. Tac.build_FSpec. Defined.
-
-Definition sigh_2 := mk_f_sigh sig_2 None None.
-Definition spec_2 : FSpec sigh_2 (fun '(p0, p1, p2) =>
-  Spec.Expanded.mk_r0 (fun '(n0, n1, n2) =>
-  Spec.Expanded.mk_r1 (GO := None) [CTX.mka (SLprop.cell p2, n2)]
-             [CTX.mka (SLprop.cell p0, n0); CTX.mka (SLprop.cell p1, n1)] True (fun p =>
-  Spec.Expanded.mk_r2 (fun '(n, n1') =>
-  Spec.Expanded.mk_r3 [CTX.mka (SLprop.cell p, n); CTX.mka (SLprop.cell p1, n1')] (n1' > 0))))).
-Proof. Tac.build_FSpec. Defined.
-
-Definition sigh_3 := mk_f_sigh sig_3 (Some (fun _ => ptr)) (Some (fun _ => ptr)).
-Definition spec_3 : FSpec sigh_3 (fun p0 p1 =>
-  Spec.Expanded.mk_r0 (fun '(n0, n1) =>
-  Spec.Expanded.mk_r1 (GO := Some _) []
-             [CTX.mka (SLprop.cell p0, n0); CTX.mka (SLprop.cell p1, n1)] True (fun r =>
-  Spec.Expanded.mk_r2 (fun '(n0', n1') =>
-  Spec.Expanded.mk_r3
-             [CTX.mka (SLprop.cell (CP.projG1 r), n0'); CTX.mka (SLprop.cell (CP.projG2 r), n1')] True)))).
-Proof. Tac.build_FSpec. Defined.
-
-Definition sigh_4 := mk_f_sigh sig_4 None (Some (fun _ => ptr)).
-Definition spec_4 : FSpec sigh_4 (fun '(p0, p1) =>
-  Spec.Expanded.mk_r0 (fun '(n0, n1) =>
-  Spec.Expanded.mk_r1 (GO := Some _) []
-             [CTX.mka (SLprop.cell p0, n0); CTX.mka (SLprop.cell p1, n1)] True (fun r =>
-  Spec.Expanded.mk_r2 (fun '(n0', n1') =>
-  Spec.Expanded.mk_r3
-             [CTX.mka (SLprop.cell (CP.projG1 r), n0'); CTX.mka (SLprop.cell (CP.projG2 r), n1')] True)))).
-Proof. Tac.build_FSpec. Defined.
-
-Definition SPEC : CP.spec_context SIG :=
-  fun f => match f with
-  | 0 => cp_f_spec (m_spec spec_0)
-  | 1 => cp_f_spec (m_spec spec_1)
-  | 2 => cp_f_spec (m_spec spec_2)
-  | 3 => cp_f_spec (m_spec spec_3)
-  | 4 => cp_f_spec (m_spec spec_4)
-  | _ => tt
-  end.
-
-Definition HSPC_f_0 := cp_has_spec SPEC f_0 eq_refl eq_refl.
-Definition HSPC_f_3 := cp_has_spec SPEC f_3 eq_refl eq_refl.
+Section Program.
+  Variables (SIG : sig_context) (SPEC : CP.spec_context SIG).
 
 
-Definition vprog_0 : f_body SPEC sigh_0 := fun '(p0, p1) =>
-  Bind _ (Read  _ p0)    (fun v0 =>
-  Bind _ (Read  _ p1)    (fun v1 =>
-  Bind _ (Write _ p0 v1) (fun _  =>
-         (Write _ p1 v0) ))).
+Definition spec_0 : FDecl (ptr * ptr) _ unit _
+  : (p0, p1)
+    FOR (n0, n1) [] [vptr p0 ~> n0; vptr p1 ~> n1] True
+    RET ( _ ) FOR tt [vptr p0 ~> n1; vptr p1 ~> n0] True.
+Proof. derive. Defined.
+Variable f_0 : spec_0 _ SPEC.
 
-Definition vprog_1 : f_body SPEC sigh_1 := fun '(p0, p1, p2) =>
-  Call _ f_0 eq_refl sigh_0 (p0, p1) tt _ (HSPC_f_0 _).
+Definition vprog_0 : FImpl f_0 := fun '(p0, p1) =>
+  'v0 <- Read p0;
+  'v1 <- Read p1;
+  Write p0 v1;;
+  Write p1 v0.
+Lemma correct_0 : FCorrect vprog_0.
+Proof. by_wlp. Qed.
+Definition cp_0: f_extract vprog_0.
+Proof. derive. Defined.
+
+
+Definition spec_1 : FDecl (ptr * ptr * ptr) _ unit _
+  : (p0, p1, p2)
+    FOR (n0, n1, n2) [vptr p2 ~> n2] [vptr p0 ~> n0; vptr p1 ~> n1] True
+    RET _ FOR tt [vptr p0 ~> n1; vptr p1 ~> n0] True.
+Proof. derive. Defined.
+Variable f_1 : spec_1 _ SPEC.
+
+Definition vprog_1 : FImpl f_1 := fun '(p0, p1, p2) =>
+  f_0 (p0, p1).
+Lemma correct_1 : FCorrect vprog_1.
+Proof. by_wlp. Qed.
+Definition cp_1: f_extract vprog_1.
+Proof. derive. Defined.
+
 
 Definition data42 : nat := 42.
 
-Definition vprog_2 : f_body SPEC sigh_2 := fun '(p0, p1, p2) =>
-  Bind _ (Read  _ p0) (fun v0 =>
-  Bind _ (Write _ p1 data42) (fun _ =>
-  Bind _ (Assert _ (fun '(v0', v1') =>
-    ([CTX.mka (SLprop.cell p0, v0'); CTX.mka (SLprop.cell p1, v1')], v0' = v0))) (fun _ =>
-  Ret _ p0 (fun p => [Vprop.mk (SLprop.cell p)])))).
+Definition spec_2 : FDecl (ptr * ptr * ptr) _ ptr _
+  : (p0, p1, p2)
+    FOR (n0, n1, n2) [vptr p2 ~> n2] [vptr p0 ~> n0; vptr p1 ~> n1] True
+    RET p FOR (n, n1') [vptr p ~> n; vptr p1 ~> n1'] (n1' > 0).
+Proof. derive. Defined.
+Variable f_2 : spec_2 _ SPEC.
 
-Definition vprog_3 : f_body SPEC sigh_3 := fun p0 p1 =>
-  Ret _ (CP.existG _ p0 p1)
-        (fun r => [Vprop.mk (SLprop.cell (CP.projG1 r)); Vprop.mk (SLprop.cell (CP.projG2 r))]).
-
-Definition vprog_4 : f_body SPEC sigh_4 := fun '(p0, p1) =>
-  Bind _ (Call _ f_3 eq_refl sigh_3 p0 p1 _ (HSPC_f_3 _)) (fun '(CP.existG _ p0' p1') =>
-  Ret _ (CP.existG _ p0' p1')
-        (fun r => [Vprop.mk (SLprop.cell (CP.projG1 r)); Vprop.mk (SLprop.cell (CP.projG2 r))])).
-
-
-Lemma imatch_0:
-  f_body_match vprog_0 (m_spec spec_0).
+Definition vprog_2 : FImpl f_2 := fun '(p0, p1, p2) =>
+  'v0 <- Read p0;
+  Write p1 data42;;
+  Assert (fun '(v0', v1') =>
+    ([vptr p0 ~> v0'; vptr p1 ~> v1'], v0' = v0));;
+  Ret p0 (pt := fun p => [Vprop.mk (vptr p)]).
+Lemma correct_2: FCorrect vprog_2.
 Proof.
-  intros (p0, p1).
-  Tac.build_impl_match.
-  FP.simpl_prog.
-  FP.by_wlp.
-  tauto.
-Qed.
-
-Definition cp_0: f_impl vprog_0.
-Proof. Tac.extract_impl. Defined.
-
-
-Lemma imatch_1:
-  f_body_match vprog_1 (m_spec spec_1).
-Proof.
-  intros ((p0, p1), p2).
-  Tac.build_impl_match.
-  FP.simpl_prog.
-  FP.by_wlp.
-  tauto.
-Qed.
-
-Definition cp_1: f_impl vprog_1.
-Proof. Tac.extract_impl. Defined.
-
-Lemma imatch_2:
-  f_body_match vprog_2 (m_spec spec_2).
-Proof.
-  intros ((p0, p1), p2).
-  Tac.build_impl_match.
-  FP.simpl_prog.
-  FP.by_wlp.
-  intuition.
+  by_wlp.
   unfold data42; repeat constructor.
 Qed.
+Definition cp_2: f_extract vprog_2.
+Proof. derive. Defined.
 
-Definition cp_2: f_impl vprog_2.
-Proof. Tac.extract_impl. Defined.
+
+Definition spec_3 : FDecl ptr (Some (fun _ => ptr)) ptr (Some (fun _ => ptr))
+  : p0 & p1
+    FOR (n0, n1) [] [vptr p0 ~> n0; vptr p1 ~> n1] True
+    RET p0' & p1' FOR (n0', n1') [vptr p0' ~> n0'; vptr p1' ~> n1'] True.
+Proof. derive. Defined.
+Variable f_3 : spec_3 _ SPEC.
+
+Definition vprog_3 : FImpl f_3 := fun p0 p1 =>
+  RetG p0 p1 (pt := fun p0 p1 => [Vprop.mk (vptr p0); Vprop.mk (vptr p1)]).
+Lemma correct_3: FCorrect vprog_3.
+Proof. by_wlp. Qed.
+Definition cp_3: f_extract vprog_3.
+Proof. derive. Defined.
 
 
-Lemma imatch_3:
-  f_body_match vprog_3 (m_spec spec_3).
+Definition spec_4 : FDecl (ptr * ptr) _ ptr (Some (fun _ => ptr))
+  : (p0, p1)
+    FOR (n0, n1) [] [vptr p0 ~> n0; vptr p1 ~> n1] True
+    RET p0' & p1' FOR (n0', n1') [vptr p0' ~> n0'; vptr p1' ~> n1'] True.
+Proof. derive. Defined.
+Variable f_4 : spec_4 _ SPEC.
+
+Definition vprog_4 : FImpl f_4 := fun '(p0, p1) =>
+  'p0' p1' <- f_3 p0 p1;
+  RetG p0' p1' (pt := fun p0 p1 => [Vprop.mk (vptr p0); Vprop.mk (vptr p1)]).
+Lemma correct_4: FCorrect vprog_4.
 Proof.
-  intros p0.
+  intro.
   Tac.build_impl_match.
   FP.simpl_prog.
-  FP.by_wlp.
+  FP.by_wlp. (* FP.by_wlp_ false. TODO FIXME*)
   tauto.
 Qed.
+Definition cp_4: f_extract vprog_4.
+Proof. derive. Defined.
 
-Definition cp_3: f_impl vprog_3.
-Proof. Tac.extract_impl. Defined.
+End Program.
 
-Lemma imatch_4:
-  f_body_match vprog_4 (m_spec spec_4).
-Proof.
-  intros (p0, p1).
-  Tac.build_impl_match.
-  FP.simpl_prog.
-  FP.by_wlp.
-  tauto.
-Qed.
+Section Extraction.
+  Definition SIG : sig_context :=
+    fun f => match f with
+    | 0 => Some (fd_sig spec_0)
+    | 1 => Some (fd_sig spec_1)
+    | 2 => Some (fd_sig spec_2)
+    | 3 => Some (fd_sig spec_3)
+    | 4 => Some (fd_sig spec_4)
+    | _ => None
+    end.
 
-Definition cp_4: f_impl vprog_4.
-Proof. Tac.extract_impl. Defined.
+  Definition SPEC : CP.spec_context SIG :=
+    fun f => match f with
+    | 0 => fd_cp spec_0
+    | 1 => fd_cp spec_1
+    | 2 => fd_cp spec_2
+    | 3 => fd_cp spec_3
+    | 4 => fd_cp spec_4
+    | _ => tt
+    end.
 
+  Definition H_f_0 := fd_mk 0 spec_0 SPEC eq_refl eq_refl.
+  Definition H_f_1 := fd_mk 1 spec_1 SPEC eq_refl eq_refl.
+  Definition H_f_2 := fd_mk 2 spec_2 SPEC eq_refl eq_refl.
+  Definition H_f_3 := fd_mk 3 spec_3 SPEC eq_refl eq_refl.
+  Definition H_f_4 := fd_mk 4 spec_4 SPEC eq_refl eq_refl.
 
-Definition IMPL : CP.impl_context SIG :=
-  fun f => match f with
-  | 0 => proj1_sig cp_0
-  | 1 => proj1_sig cp_1
-  | 2 => proj1_sig cp_2
-  | 3 => proj1_sig cp_3
-  | 4 => proj1_sig cp_4
-  | _ => tt
-  end.
+  Definition IMPL : CP.impl_context SIG :=
+    fun f => match f with
+    | 0 => proj1_sig (cp_0 _ _ H_f_0)
+    | 1 => proj1_sig (cp_1 _ _ H_f_0 H_f_1)
+    | 2 => proj1_sig (cp_2 _ _ H_f_2)
+    | 3 => proj1_sig (cp_3 _ _ H_f_3)
+    | 4 => proj1_sig (cp_4 _ _ H_f_3 H_f_4)
+    | _ => tt
+    end.
 
-Ltac case_until_True :=
-  try exact (fun _ => Logic.I);
-  let i := fresh "i" in
-  intros [|i]; [|revert i; case_until_True].
+  Ltac case_until_True :=
+    try exact (fun _ => Logic.I);
+    let i := fresh "i" in
+    intros [|i]; [|revert i; case_until_True].
 
-Lemma match_context:
-  CP.context_match_spec IMPL SPEC.
-Proof.
-  case_until_True;
-  cbn beta iota delta [SIG IMPL SPEC];
-  apply f_impl_match_spec.
-  - apply imatch_0.
-  - apply imatch_1.
-  - apply imatch_2.
-  - apply imatch_3.
-  - apply imatch_4.
-Qed.
+  Lemma match_context:
+    CP.context_match_spec IMPL SPEC.
+  Proof.
+    case_until_True;
+    cbn beta iota delta [SIG IMPL SPEC];
+    apply f_extract_match_spec.
+    - apply correct_0.
+    - apply correct_1.
+    - apply correct_2.
+    - apply correct_3.
+    - apply correct_4.
+  Qed.
 
-Lemma context_oracle_free:
-  CP.context_oracle_free IMPL.
-Proof.
-  case_until_True;
-  cbn beta iota delta [SIG IMPL SPEC];
-  apply f_impl_oracle_free.
-Qed.
+  Lemma context_oracle_free:
+    CP.context_oracle_free IMPL.
+  Proof.
+    case_until_True;
+    cbn beta iota delta [SIG IMPL SPEC];
+    apply f_extract_oracle_free.
+  Qed.
+End Extraction.
 
+Section Other.
 
 Definition sigh_a0 := mk_f_sig1 (ptr * ptr) None unit None.
-Definition spec_a0 : FSpec sigh_a0 (fun ps =>
-  Spec.Expanded.mk_r0 (fun n =>
-  Spec.Expanded.mk_r1 [CTX.mka (SLprop.cell (fst ps), n)] [] True (fun _ =>
-  Spec.Expanded.mk_r2 (fun 'tt =>
-  Spec.Expanded.mk_r3 [] True)))).
+Definition spec_a0 : FSpec sigh_a0
+  : ps
+    FOR n [vptr (fst ps) ~> n] [] True
+    RET _ FOR tt [] True.
 Proof. Tac.build_FSpec. Defined.
 
 Definition vprog_a0 : f_body SPEC sigh_a0 := fun ps =>
-  Bind _ (let (p0, _) := ps in Read _ p0) (fun v0 =>
-  Ret _ tt (fun _ => [])).
+  'v0 <- let (p0, _) := ps in Read p0;
+  Ret tt.
 Lemma imatch_a0:
   f_body_match vprog_a0 (m_spec spec_a0).
 Proof.
@@ -245,24 +194,21 @@ Proof.
   cbn. tauto.
 Qed.
 
-Definition cp_a0: f_impl vprog_a0.
+Definition cp_a0: f_extract vprog_a0.
 Proof. Tac.extract_impl. Defined.
 
 
 Definition sigh_a1a := mk_f_sig1 (bool * ptr * ptr * ptr) None unit None.
-Definition spec_a1a : FSpec sigh_a1a (fun '(b, p0, p1, p2) =>
-  Spec.Expanded.mk_r0 (fun '(n0, n1, n2) =>
-  Spec.Expanded.mk_r1 [CTX.mka (SLprop.cell p0, n0)] [CTX.mka (SLprop.cell p1, n1); CTX.mka (SLprop.cell p2, n2)]
-    True (fun _ =>
-  Spec.Expanded.mk_r2 (fun '(n1', n2') =>
-  Spec.Expanded.mk_r3 [CTX.mka (SLprop.cell p1, n1'); CTX.mka (SLprop.cell p2, n2')]
-    (b = true -> n1' = 0))))).
+Definition spec_a1a : FSpec sigh_a1a
+  : (b, p0, p1, p2)
+    FOR (n0, n1, n2) [vptr p0 ~> n0] [vptr p1 ~> n1; vptr p2 ~> n2] True
+    RET _ FOR (n1', n2') [vptr p1 ~> n1'; vptr p2 ~> n2'] (b = true -> n1' = 0).
 Proof. Tac.build_FSpec. Defined.
 
 Definition vprog_a1a : f_body SPEC sigh_a1a := fun '(b, p0, p1, p2) =>
   if b
-  then Write _ p1 0
-  else Write _ p2 1.
+  then Write p1 0
+  else Write p2 1.
 Lemma imatch_a1a:
   f_body_match vprog_a1a (m_spec spec_a1a).
 Proof.
@@ -273,24 +219,23 @@ Proof.
   intuition congruence.
 Qed.
 
-Definition cp_a1a: f_impl vprog_a1a.
+Definition cp_a1a: f_extract vprog_a1a.
 Proof. Tac.extract_impl. Defined.
 
 
 Inductive bool3 : Set := B0 | B1 | B2.
 
 Definition sigh_a1b := mk_f_sig1 (bool3 * ptr) None unit None.
-Definition spec_a1b : FSpec sigh_a1b (fun '(b, p) =>
-  Spec.Expanded.mk_r0 (fun n =>
-  Spec.Expanded.mk_r1 [] [CTX.mka (SLprop.cell p, n)] (b <> B2) (fun _ =>
-  Spec.Expanded.mk_r2 (fun n' =>
-  Spec.Expanded.mk_r3 [CTX.mka (SLprop.cell p, n')] (b <> B1 -> n' = 0))))).
+Definition spec_a1b : FSpec sigh_a1b
+  : (b, p)
+    FOR n [] [vptr p ~> n] (b <> B2)
+    RET _ FOR n' [vptr p ~> n'] (b <> B1 -> n' = 0).
 Proof. Tac.build_FSpec. Defined.
 
 Definition vprog_a1b : f_body SPEC sigh_a1b := fun '(b, p) =>
   match b with
-  | B0 => Write _ p 0
-  | B1 | B2 => Ret _ tt (fun _ => [])
+  | B0 => Write p 0
+  | B1 | B2 => Ret tt
   end.
 Lemma imatch_a1b:
   f_body_match vprog_a1b (m_spec spec_a1b).
@@ -304,18 +249,16 @@ Qed.
 
 
 Definition sigh_a1c := mk_f_sig1 (option nat * ptr) None unit None.
-Definition spec_a1c : FSpec sigh_a1c (fun '(o, p) =>
-  Spec.Expanded.mk_r0 (fun n =>
-  Spec.Expanded.mk_r1 [] [CTX.mka (SLprop.cell p, n)]
-    (n > 0 /\ match o with Some n' => n' > 0 | None => True end) (fun _ =>
-  Spec.Expanded.mk_r2 (fun n' =>
-  Spec.Expanded.mk_r3 [CTX.mka (SLprop.cell p, n')] (n' > 0))))).
+Definition spec_a1c : FSpec sigh_a1c
+  : (o, p)
+    FOR n [] [vptr p ~> n] (n > 0 /\ match o with Some n' => n' > 0 | None => True end)
+    RET _ FOR n' [vptr p ~> n'] (n' > 0).
 Proof. Tac.build_FSpec. Defined.
 
 Definition vprog_a1c : f_body SPEC sigh_a1c := fun '(o, p) =>
   match o with
-  | Some n => Write _ p n
-  | None   => Ret _ tt (fun _ => [])
+  | Some n => Write p n
+  | None   => Ret tt
   end.
 Lemma imatch_a1c:
   f_body_match vprog_a1c (m_spec spec_a1c).
@@ -329,19 +272,17 @@ Qed.
 
 
 Definition sigh_a2a := mk_f_sig1 (ptr * ptr) None unit None.
-Definition spec_a2a : FSpec sigh_a2a (fun '(p0, p1) =>
-  Spec.Expanded.mk_r0 (fun '(n0, n1) =>
-  Spec.Expanded.mk_r1 [CTX.mka (SLprop.cell p0, n0)] [CTX.mka (SLprop.cell p1, n1)]
-    (n0 <= n1) (fun _ =>
-  Spec.Expanded.mk_r2 (fun n1' =>
-  Spec.Expanded.mk_r3 [CTX.mka (SLprop.cell p1, n1')] (n0 <= n1'))))).
+Definition spec_a2a : FSpec sigh_a2a
+  : (p0, p1)
+    FOR (n0, n1) [vptr p0 ~> n0] [vptr p1 ~> n1] (n0 <= n1)
+    RET _ FOR n1' [vptr p1 ~> n1'] (n0 <= n1').
 Proof. Tac.build_FSpec. Defined.
 
 Definition vprog_a2a : f_body SPEC sigh_a2a := fun '(p0, p1) =>
-  Bind _ (Read _ p1) (fun v1 =>
-  Bind _ (GGet _ (SLprop.cell p0)) (fun v0 =>
-  Bind _ (Assert _ (fun 'tt => ([], v0 <= v1))) (fun _ =>
-          Write _ p1 (S v1)))).
+  'v1 <- Read p1;
+  'v0 <- GGet (SLprop.cell p0);
+  Assert (fun 'tt => ([], v0 <= v1));;
+  Write p1 (S v1).
 Lemma imatch_a2a:
   f_body_match vprog_a2a (m_spec spec_a2a).
 Proof.
@@ -351,15 +292,16 @@ Proof.
   FP.by_wlp.
   intuition.
 Qed.
-Definition cp_a2a: f_impl vprog_a2a.
+Definition cp_a2a: f_extract vprog_a2a.
 Proof. Tac.extract_impl. Defined.
 
 Definition vprog_a2b : f_body SPEC sigh_a2a := fun '(p0, p1) =>
-  Bind _ (Bind _ (Read _ p1) (fun v1 =>
-          Bind _ (GGet _ (SLprop.cell p0)) (fun v0 =>
-          Ret _ (CP.existG _ v1 v0) (fun _ => [])))) (fun '(CP.existG _ v1 v0) =>
-  Bind _ (Assert _ (fun 'tt => ([], v0 <= v1))) (fun _ =>
-          Write _ p1 (S v1))).
+  'v1 v0 <- (
+    'v1 <- Read p1;
+    'v0 <- GGet (SLprop.cell p0);
+    RetG v1 v0);
+  Assert (fun 'tt => ([], v0 <= v1));;
+  Write p1 (S v1).
 Lemma imatch_a2b:
   f_body_match vprog_a2b (m_spec spec_a2a).
 Proof.
@@ -369,20 +311,19 @@ Proof.
   FP.by_wlp.
   intuition.
 Qed.
-Definition cp_a2b: f_impl vprog_a2b.
+Definition cp_a2b: f_extract vprog_a2b.
 Proof. Tac.extract_impl. Defined.
 
 
 Definition sigh_a3 := mk_f_sig1 unit (Some (fun _ => (nat * nat)%type <: Type)) unit (Some (fun _ => nat <: Type)).
-Definition spec_a3 : FSpec sigh_a3 (fun _ '(n0, n1) =>
-  Spec.Expanded.mk_r0 (fun 'tt =>
-  Spec.Expanded.mk_r1 (GO := Some _) [] [] True (fun r =>
-  Spec.Expanded.mk_r2 (fun 'tt =>
-  Spec.Expanded.mk_r3 [] (CP.projG2 r = n0 + n1))))).
+Definition spec_a3 : FSpec sigh_a3
+  : _ & (n0, n1)
+    FOR tt [] [] True
+    RET _ & r FOR tt [] (r = n0 + n1).
 Proof. Tac.build_FSpec. Defined.
 
 Definition vprog_a3 : f_body SPEC sigh_a3 := fun _ '(n0, n1) =>
-  Ret _ (CP.existG _ tt (n0 + n1)) (fun _ => []).
+  RetG tt (n0 + n1).
 Lemma imatch_a3:
   f_body_match vprog_a3 (m_spec spec_a3).
 Proof.
@@ -392,5 +333,6 @@ Proof.
   FP.by_wlp.
   tauto.
 Qed.
-Definition cp_a3: f_impl vprog_a3.
+Definition cp_a3: f_extract vprog_a3.
 Proof. Tac.extract_impl. Defined.
+End Other.
